Progress on IG dfs terminantion

project/inductive/inductive_graph.v
@@ -100,12 +100,13 @@ Definition _cleanSplit {A B : Type} (node : Node) (context' : Context' A B) (ig 
   match context' with
   | (froms, label, tos) =>
                           let rmLoops :=  filter (fun '(_, n) => negb (n =? node)) in
+
                           let froms' := rmLoops froms in
                           let tos' := rmLoops tos in
                           let context := (froms', node, label, tos (*no '*)) in
                           
-                          let ig' := _updAdj froms' (fun x y => _clearPred node y) ig in
-                          let ig'' := _updAdj tos' (fun x y => _clearSucc node y) ig' in
+                          let ig' := _updAdj froms' (fun x y => _clearSucc node y) ig in 
+                          let ig'' := _updAdj tos' (fun x y => _clearPred node y) ig' in
                           (context, ig'')
   end.
 
@@ -143,8 +144,6 @@ Definition insNodes {A B : Type} (nodes : list (LNode A)) (ig : IG A B) : IG A B
 
 
 
-
-
 Definition insEdge {A B : Type} (edge : LEdge B) (ig : IG A B) : IG A B :=
   match edge with
   | (from, to, l) =>
@@ -154,33 +153,488 @@ Definition insEdge {A B : Type} (edge : LEdge B) (ig : IG A B) : IG A B :=
                     | None => ig
                     end
   end.
-                    
+
+
 Definition insEdges {A B : Type} (edges : list (LEdge B)) (ig : IG A B) : IG A B :=
   fold_right insEdge ig edges.
 
 
 
-Definition mkGraph {A B : Type} (nodes : list (LNode A)) (edges : list (LEdge B)) : IG A B :=
+Definition IG_mkGraph {A B : Type} (nodes : list (LNode A)) (edges : list (LEdge B)) : IG A B :=
   insEdges edges (insNodes nodes IG_empty).
 
  
-Definition labNodes {A B : Type} (ig : IG A B) : list (LNode A) :=
+Definition IG_labNodes {A B : Type} (ig : IG A B) : list (LNode A) :=
   map (fun '(v, (_, l, _)) => (v,l)) (NatMap.elements ig).
-
-
-
-
-
 
 
 
 (* Make IGs visible  *)
 
-Definition show_IG {A B : Type} (ig : IG A B) :=
+Definition IG_show {A B : Type} (ig : IG A B) :=
   NatMap.elements ig. 
 
-Definition show_Decomp {A B : Type} (d : Decomp A B) :=
+Definition Decomp_show {A B : Type} (d : Decomp A B) := 
   match d with
-  | (mContext, x) => (mContext, show_IG x)
+  | (mContext, x) => (mContext, IG_show x)
   end
 .
+
+
+
+(* Now come some more advanced operations *)
+
+(* Auxiliary graph class functions: *)
+Definition IG_matchAny {A B : Type} (ig : IG A B) : Decomp A B :=
+  match IG_labNodes ig with
+  | [] => (None, ig)
+  | node :: nodes => IG_match (fst node)  ig
+  end.
+  
+
+
+Definition IG_noNodes {A B : Type} (ig : IG A B) : nat :=
+  length (IG_labNodes ig).
+
+Definition _minimum (l : list nat) : nat :=
+  fold_right min 0 l.
+
+(* This is a hack *)
+Definition _maximum (l : list nat) : nat :=
+  fold_right max 1000 l.
+
+Definition IG_nodeRange {A B : Type} (ig : IG A B) : Node * Node :=
+  match IG_isEmpty ig with
+  | true => (0, 0)
+  | false =>
+    let nodes := map fst (IG_labNodes ig) in
+    (_minimum nodes, _maximum nodes)
+  end.
+    
+
+
+Definition IG_labEdges {A B : Type} (ig : IG A B) : list (LEdge B) :=
+  fold_right (fun '(node, (_, _, tos)) acc => map (fun '(l, to) => (node, to, l)) tos ++ acc) [] (NatMap.elements ig). 
+
+
+
+(* Here stars DFS stuff *)
+
+
+
+Definition suc {A B : Type} (c : Context A B) : list Node :=
+  match c with
+  | (_, _, _, tos) => map snd tos
+  end.
+
+Fixpoint IG_dfs_fuled {A B : Type} (nodes : list Node) (ig : IG A B) (fuel : nat) : list Node :=
+  match fuel with
+  | 0 => []
+  | S fuel' =>
+    match nodes with
+    | [] => []
+    | n :: ns => if IG_isEmpty ig then [] else
+                  match IG_match n ig with
+                  | (Some cntxt, rest) => n :: IG_dfs_fuled (suc cntxt ++ ns) rest fuel'
+                  | (None, same) => IG_dfs_fuled ns same fuel'
+                  end
+    end
+  end.
+Definition my_complicated_graph :=
+  IG_mkGraph
+    [(1, "a"); (2, "b"); (3, "c"); (4, "d"); (5, "e"); (6, "f")]
+    [ (1, 2, "edge1");
+      (2, 3, "edge2");
+      (3, 1, "edge3");
+      (2, 4, "edge4");
+      (4, 5, "edge5");
+      (5, 6, "edge6");
+      (6, 3, "edge7");
+      (1, 5, "edge8");
+      (6, 1, "edge9")]
+.
+
+Compute IG_dfs_fuled [1] my_complicated_graph 50.
+
+
+
+
+
+
+
+
+
+
+
+(* https://fzn.fr/teaching/coq/ecole10/summer/lectures/lec10.pdf *)
+
+  
+
+Require Import Coq.Arith.Arith.
+Require Import Coq.Arith.Wf_nat.
+Require Import Coq.Init.Nat.
+Require Import Coq.Lists.List.
+Require Import Coq.Program.Wf.
+Require Import Coq.Wellfounded.Wellfounded.
+Require Import Coq.Wellfounded.Lexicographic_Product.
+Require Import Coq.Structures.OrderedType.
+Require Import Coq.Structures.OrderedTypeEx.
+Require Import Recdef. (* Must import this to use the Function feature *)
+
+Import ListNotations.
+Require Import Coq.Wellfounded.Inverse_Image.
+
+
+
+
+Definition dProdDfs (A B : Type) := {_ : list Node & IG A B}.
+
+(* Lexicographic order on (nat * nat) *)
+Definition lex_dProdDfs (A B : Type) := Relation_Operators.lexprod (list Node)
+                                                (fun a => IG A B)
+                                                (fun l1 l2 => Peano.lt (length l1) (length l2))
+                                                (fun a:list Node => fun ig1 ig2 => Peano.lt (NatMap.cardinal ig1) (NatMap.cardinal ig2)). 
+
+
+(* Prove lexicographic order is well-founded *)
+Lemma wf_lex_dProdDfs (A B : Type) : well_founded (lex_dProdDfs A B).
+Proof.
+  apply wf_lexprod.
+  - apply well_founded_ltof. 
+  - intros. apply well_founded_ltof.
+Qed.
+
+
+
+
+
+Definition prodTodPairDfs {A B : Type} (p : list Node * IG A B) : dProdDfs A B :=
+  existT _ (fst p) (snd p).
+
+Definition lex_prodDfs (A B : Type) (nodesIg1 nodesIg2 : list Node * IG A B) : Prop := 
+  lex_dProdDfs _ _ (prodTodPairDfs nodesIg1) (prodTodPairDfs nodesIg2).
+
+
+(* Prove lexicographic order is well-founded *)
+Lemma wf_lex_prodDfs (A B : Type) : well_founded (lex_prodDfs A B).
+Proof.
+  unfold lex_prodDfs.
+  pose proof (wf_lex_dProdDfs A B).
+  pose proof (wf_inverse_image (list Node * IG A B) _ (lex_dProdDfs A B)).
+
+  apply (H0 (@prodTodPairDfs A B)) in H.
+  assumption.
+Qed.
+
+
+
+
+
+
+
+Function IG_dfs' {A B : Type} (nodesIg : list Node * IG A B) {wf (lex_prodDfs A B) nodesIg} : list Node := 
+  match nodesIg with
+  | (nodes, ig) =>
+    match nodes with
+    | [] => []
+    | n :: ns => if IG_isEmpty ig then [] else
+                  match IG_match n ig with
+                  | (Some cntxt, rest) => n :: IG_dfs' ((suc cntxt ++ ns), rest)
+                  | (None, same) => IG_dfs' (ns, same)
+                  end
+    end
+  end.
+Proof.
+  - admit.
+  - admit.
+  - apply  wf_lex_prodDfs.
+Admitted.
+
+
+
+
+
+
+
+
+
+
+
+
+
+
+
+(* Vanilla version: *)
+Fixpoint IG_dfs {A B : Type} (nodes : list Node) (ig : IG A B) : list Node :=
+  match nodes with
+  | [] => []
+  | n :: ns => if IG_isEmpty ig then [] else
+                match IG_match n ig with
+                | (Some cntxt, rest) => n :: IG_dfs (suc cntxt ++ ns) rest
+                | (None, same) => IG_dfs ns same
+                end
+  end.
+Proof.
+- intros. Admitted.
+
+
+
+
+
+
+
+
+
+
+
+
+
+
+
+
+
+
+
+
+
+
+
+
+
+
+
+
+
+
+
+(* 
+(* Here starts stuff from the paper, that I did not bother to implement *)
+Require Import Recdef. (* Must import this to use the Function feature *)
+
+Function IG_gmap {A B C D : Type} (f : IG_Context A B -> IG_Context C D) (ig : IG A B) {measure IG_measure ig} : IG C D :=
+  match IG_matchAny ig with
+    | ((True, c), rest) => _add (f c) (IG_gmap f rest)
+    (* | ((False, c), rest) => _add (f c) (IG_gmap f rest) *)
+  end
+.
+Proof. Admitted.
+
+
+
+Definition IG_grev {A B : Type} (ig : IG A B) : IG A B :=
+  IG_gmap _ _ _ _ (fun '((froms, node, tos) : IG_Context A B) => (tos, node, froms)) ig
+.
+
+Function IG_ufold {A B C : Type} (f : IG_Context A B -> C -> C) (acc : C) (ig : IG A B) {measure IG_measure ig} : C :=
+  match IG_matchAny ig with
+    | ((True, c), rest) => f c (IG_ufold f acc rest)
+    (* | ((False, c), rest) => _add (f c) (IG_gmap f rest) *)
+  end
+.
+Proof. Admitted.
+
+
+Definition IG_gmap' {A B C D : Type} (f : IG_Context A B -> IG_Context C D) (ig : IG A B) : IG C D :=
+  IG_ufold _ _ (IG C D) (fun (c : IG_Context A B) (acc : IG C D) => _add (f c) acc) IG_empty ig.
+
+
+Definition IG_nodes' {A B : Type} (ig : IG A B) : list A :=
+  IG_ufold _ _ _ (fun '(froms, node, tos) acc => node :: acc ) [] ig.
+  
+Definition IG_undir {A B : Type} (ig : IG A B) : IG A B :=
+  IG_gmap _ _ _ _ (fun '(froms, node, tos) =>
+    let fromsTos := (fun (b : B) (a : A) => froms b a \/ tos b a) in
+    (fromsTos, node, fromsTos)) ig
+.
+
+Definition IG_gsuc {A B : Type} (node : A) (ig : IG A B) : Ensemble A :=
+  match IG_match node ig with
+    | ((True, (_, _, tos)), rest) => fun (a : A) => exists l, tos l a 
+  end
+.
+
+(* IG_deg is hard to implement, as is is hard to count *)
+Definition IG_deg {A B : Type} (node : A) (ig : IG A B) : nat.
+Proof. Admitted.
+(* :=
+  match IG_match node ig with
+    | ((True, (froms, nodeAgain, tos)), rest) => fun (a : A) => CARDINALITY froms tos 
+  end
+. *)
+
+Definition IG_del {A B : Type} (node : A) (ig : IG A B) : IG A B :=
+  match IG_match node ig with
+    | ((True, _), rest) => rest
+  end
+.
+
+Definition IG_suc {A B : Type} (node : A) (c : IG_Context A B) : Ensemble A :=
+  match c with | (_, _, tos) =>
+    fun (a : A) => exists l, tos l a 
+  end
+.
+
+
+
+(* More advanced stuff *)
+
+dfs :: [Node] → Graph a b → [Node]
+dfs [ ]
+g
+= []
+v
+dfs (v :vs) (c & g) = v :dfs (suc c++vs) g
+dfs (v :vs) g
+= dfs vs g
+
+(* Possible extensions: *)
+dfs vs Empty = [ ]
+dfs vs g | null vs || isEmpty g = [ ]
+
+
+dfs [ ]
+g0 = [ ]
+dfs (v :vs) g 0 = case match v g 0 of
+(Just c, g) → v :dfs (suc c++vs) g
+(Nothing, g) → dfs vs g
+
+data Tree a = Br a [Tree a]
+postorder :: Tree a → [a]
+postorder (Br v ts) = concatMap postorder ts++[v ]
+
+concatMap :: (a → [b]) → [a] → [b]
+concatMap f = concat . map f
+
+
+df :: [Node] → Graph a b → ([Tree Node], Graph a b)
+df [ ]
+g
+= ([ ], g)
+v
+df (v :vs) (c & g) = (Br v f :f 0 , g2 ) where (f , g1 ) = df (suc c) g
+(f 0 , g2 ) = df vs g1
+df (v :vs) g
+= df vs g
+
+dff :: [Node] → Graph a b → [Tree Node]
+dff vs g = fst (df vs g)
+
+
+topsort :: Graph a b → [Node]
+topsort = reverse . concatMap postorder . dff
+scc :: Graph a b → [Tree Node]
+scc g = dff (topsort g) (grev g)
+
+
+
+
+(* BFS *)
+
+bfs :: [Node] → Graph a b → [Node]
+bfs [ ]
+g
+= []
+v
+bfs (v :vs) (c & g) = v :bfs (vs++suc c) g
+bfs (v :vs) g
+= bfs vs g
+
+type Path = [Node]
+type RTree = [Path]
+bft :: Node → Graph a b → RTree
+bft v = bf [[v ]]
+bf :: [Path] → Graph a b → RTree
+bf [ ]
+g
+= []
+v
+bf (p@(v : ):ps) (c & g) = p:bf (ps++map (:p) (suc c)) g
+bf (p:ps)
+g
+= bf ps g
+
+
+first :: (a → Bool ) → [a] → a
+first p = head . filter p
+esp :: Node → Node → Graph a b → Path
+esp s t = reverse . first (\(v : ) → v t) . bft s
+
+
+(* Shortest path: *)
+
+type LNode a = (Node, a)
+type LPath a = [LNode a]
+type LRTree a = [LPath a]
+instance Eq a ⇒ Eq (LPath a) where
+(( , x ): ) (( , y): ) = x y
+instance Ord a ⇒ Ord (LPath a) where
+(( , x ): ) < (( , y): ) = x < y
+getPath :: Node → LRTree a → Path
+getPath v = reverse . map fst . first (\((w , ): ) → w == v)
+
+
+
+expand :: Real b ⇒ b → LPath b → Context a b → [Heap (LPath b)]
+expand d p ( , , , s) = map (\(l , v ) → unitHeap ((v , l + d ):p)) s
+dijkstra :: Real b ⇒ Heap (LPath b) → Graph a b → LRTree b
+dijkstra h g | isEmptyHeap h || isEmpty g = [ ]
+v
+dijkstra (p@((v , d ): )≺h) (c & g) = p:dijkstra (meigeAll (h:expand d p c)) g
+dijkstra ( ≺h) g
+= dijkstra h g
+
+
+
+
+spt :: Real b ⇒ Node → Graph a b → LRTree b
+spt v = spt (unitHeap [(v , 0)])
+sp :: Real b ⇒ Node → Node → Graph a b → Path
+sp s t = getPath t . spt s
+
+
+
+(* Minimum spanning tree *)
+addEdges :: Real b ⇒ LPath b → Context a b → [Heap (LPath b)]
+addEdges p ( , , , s) = map (\(l , v ) → unitHeap ((v , l ):p)) s
+
+mst :: Real b ⇒ Node → Graph a b → LRTree b
+mst v g = prim (unitHeap [(v , 0)]) g
+prim :: Real b ⇒ Heap (LPath b) → Graph a b → LRTree b
+prim h g | isEmptyHeap h || isEmpty g = [ ]
+v
+prim (p@((v , ): )≺h) (c & g) = p:prim (meigeAll (h:addEdges p c)) g
+prim ( ≺h) g
+= prim h g
+
+mstp :: Real b ⇒ LRTree b → Node → Node → Path
+mstp t a b = joinPaths (getPath a t) (getPath b t)
+joinPaths :: Path → Path → Path
+joinPaths p q = joinAt (head p) (tail p) (tail q)
+joinAt :: Node → Path → Path → Path
+joinAt x (v :vs) (w :ws) | v w = joinAt v vs ws
+joinAt x p
+q
+= reverse p++(x :q)
+
+
+
+(* Maximum independent node set: *)
+
+
+indep :: Graph a b → [Node]
+indep Empty = [ ]
+indep g
+= if length i1 > length i2 then i1 else i2
+where vs
+= nodes g
+m
+= maximum (map (flip deg g) vs)
+v
+= first (\v → deg v g m) vs
+v
+c & g0 = g
+i1
+= indep g 0
+i2
+= v :indep (foldr del g 0 (pre c++suc c))
+ *)
