project/inductive/inductive_graph_to_RG.v
@@ -10,44 +10,61 @@ Require Import MyProject.project.inductive.inductive_graph.
 Require Import MyProject.project.relational_graph.
 Require Import MyProject.project.relational_graph_theory.
 
+Require Import MyProject.project.util.NatMap.
+Require Import MyProject.project.util.NatSet.
+Require Import MyProject.project.util.util.
 
-(* Defining Conversion from Inductive Graph to Relational Graph, this is a work in progress *)
+(* Defining Conversion from Inductive Graph to Relational Graph *)
 
- 
 
-Definition labEdges {A B : Type} (ig : IG A B) : list (LEdge B).
+(* Adds a node and its in- and out- going edges (= its IG context) to an RG.
+    Adds the neighbouring nodes, in case they do not exists *)
+Definition _extendByContext {B : Type} (node : Node) (froms tos : Adj B) (rg : RG_unlE nat) : RG_unlE nat.
 Proof.
-Admitted. 
-
-Definition IG_to_RG {A B : Type} (ig : IG A B) : RG A B.
-Proof.
-    Print labNodes.
-    (* list of node labels *)
-    pose (nodes := map snd (labNodes ig)).
-    (* list of connections made by edges (drop labels)*)
-    pose (edges := map (fun (edge : LEdge B) => match edge with | (from, to, lab) => (lookup from ig, lookup to ig) end) (labEdges ig)).
-    
     refine {|
-        RG_nodes := fun (a : A) =>
-                            fold_right (fun (v : A) (acc: Prop) => (a = v) \/ acc) False nodes;
-(* This is wrong now, that there are edge labels to consider *)
-        RG_edges := fun (a1 a2 : A) l =>
-                            fold_right (fun (e : (option A) * (option A)) (acc: Prop) => match e with
-                                | (Some from, Some to) => ((a1 = from) /\ (a2 = to)) \/ acc
-                                (* This case should never happen *)
-                                | _ => acc
-                                end) False edges;
+        RG_nodes := fun (n : nat) => In n (map snd froms) \/ In n (map snd tos) \/ (cEnsembleAdd node rg.(RG_nodes)) n; 
+        RG_edges := fun (n1 n2 : nat) l =>
+                                (In n1 (map snd froms) /\ n2 = node)
+                                \/ (n1 = node /\ In n2 (map snd tos))
+                                \/ rg.(RG_edges) n1 n2 l
+                                ;
                      
         RG_valid := _
     |}.
-    RG_valid_prover.
-Admitted.
+    RG_valid_prover_with rg.
+Defined.
 
 
-Coercion IG_to_RG : IG >-> RG.
+(* Adds a node and its in- and out- going edges (= its IG context) to an RG.
+    Assumes that the neighboring nodes exist *)
+Definition _accTo_RG_unlE {A B : Type} (node : LNode A) (rgIg : RG_unlE nat * IG A B) : RG_unlE nat * IG A B :=
+    match node with
+    | (node, lab) =>
+        match rgIg with
+        | (rg, ig) =>
+            match IG_match node ig with
+            | (Some (froms, _, _, tos), rest) => (_extendByContext node froms tos rg, rest)
+            | (None, sameIg)            => (rg, sameIg)
+            end
+        end
+    end
+.
+
+(* Looses multi-edges (IGs can have multiple same-label edges), Also looses labels *)
+Definition IG_to_RG {A B : Type} (ig : IG A B) : RG_unlE nat :=
+    match fold_right _accTo_RG_unlE (RG_empty, ig) (IG_labNodes ig) with
+    | (rg, acc) => rg
+    end
+.
 
 
-Definition IG_equiv {A : Type} (ig1 ig2 : IG A unit) : Prop :=
-    RG_equiv ig1 ig2.
+(* Coercion IG_basic_to_RG : IG_basic >-> RG. *)
+
+(* This does not respect the labels for now *)
+Definition IG_equiv {A B : Type} (ig1 ig2 : IG A B) : Prop :=
+    RG_equiv (IG_to_RG ig1) (IG_to_RG ig2)
+.
 
 Notation "g1 I== g2" := (IG_equiv g1 g2) (at level 80).
+
+
