project/inductive/inductive_graph_theory.v
@@ -1,68 +1,256 @@
-Require Import String.
+(* Require Import Coq.micromega.Lia.
+Require Import Coq.Logic.FunctionalExtensionality.
+Require Import Coq.Logic.PropExtensionality.
+
 Require Import Coq.Arith.Arith.
 
 Require Import List.
+Require Import Coq.Structures.OrdersTac.
 Require Import Bool.
 Import ListNotations.
+
+Require Import FSets.
+Require Import FMaps.
+Require Import OrderedTypeEx.
 Require Import Setoid Morphisms.
 
 
-Require Import MyProject.project.relational_graph.
-Require Import MyProject.project.relational_graph_theory.
+Require Import MyProject.project.util.NatSet.
 
 Require Import MyProject.project.inductive.inductive_graph.
 Require Import MyProject.project.inductive.inductive_graph_to_RG.
 
-Open Scope nat_scope.
+Require Import MyProject.project.relational_graph.
+Require Import MyProject.project.relational_graph_theory.
+
+(* This file shows that I== is an equivalence and attempts at "direct equational specification" of IG s  *)
 
 
 (* Section to make rewrite work with IG_equiv *)
 (* This proof is based on === being an equivalence relation *)
-Instance IG_Equivalence {A : Type} : Equivalence (@IG_equiv A).
+Instance IG_Equivalence {A B : Type} : Equivalence (@IG_equiv A B).
 Proof.
-    G_derived_equivalence_prover A unit (@id (IG A unit)).
-Qed. 
-
-
-Example basic_equivalence_test : (mkGraph [(1, "1"); (2, "2")] []) I== (mkGraph [(2, "2"); (1, "1")] []).
-Proof.
-  unfold IG_equiv. unfold RG_equiv. simpl. split; split; intros.
-  - admit.
-  - admit.
-  - admit.
-  - admit.
-Admitted.
-
-
+  G_derived_equivalence_prover nat unit (@ IG_to_RG A B).  
+Qed.
 
 
 (* (attempt at) direct equational specifications of an IG: *)
 
+(* Block to derive useful conversion theorem "In_labNodes_is_InMap" *)
 
-Theorem spec1 : forall A B, isEmpty (@empty A B) = true.
+
+(* Helper lemma for converting an In (of a map) to an InA, which will eventually be turned to a NatMap.In (which has useful lemmas)  *)
+Lemma _In_map_fst_InA : forall (A B: Type) (a : A) (l : list (A * B)),
+  In a (map fst l) <-> exists (a0 : B), InA (fun (x el : (A * B)) => x = el) (a, a0) l.
+Proof.
+  intros. induction l; simpl.
+  - split; intros.
+    + destruct H.
+    + destruct H. inversion H.
+  - split; intros.
+    + destruct H.
+      -- exists (snd a0). left. destruct a0. destruct H. simpl. reflexivity.
+      -- edestruct IHl. apply H0 in H. destruct H. exists x. apply InA_cons. right. assumption.
+    + destruct H. inversion H.
+      -- left. destruct a0. destruct H1. simpl. reflexivity.
+      -- right. apply IHl. exists x. assumption.
+Qed.  
+
+
+
+(* Conversion from key equality from map to my own (simply written in a slightly different manner) *)
+Lemma _In_conditions_same : (NatMap.eq_key_elt (elt:=NatSet.t * NatSet.t)) = (fun x el : Node * (NatSet.t * NatSet.t) => x = el).
+Proof.
+  unfold NatMap.eq_key_elt. unfold NatMap.Raw.PX.eqke.
+  apply functional_extensionality.
+  intros.
+  apply functional_extensionality.
+  intros.
+  destruct x, x0.
+  simpl.
+  apply propositional_extensionality.
+  split; intros.
+  - destruct H. subst. reflexivity.
+  - inversion H. auto.
+Qed.
+
+(* This is the most useful one for proving other statements.
+  Use it to convert from "use friendly" In- statements to "provable" NatMap.In- statements  *)
+Lemma _In_labNodes_is_InMap : forall (x : Node) (ig : IG),
+  In x (IG_labNodes ig) <-> NatMap.In x ig.
+Proof.
+  intros. unfold IG_labNodes.
+  rewrite _In_map_fst_InA.
+  pose proof (WF.elements_in_iff ig).
+  rewrite _In_conditions_same in H.
+  specialize H with x.
+  symmetry.
+  assumption.
+Qed.
+
+
+(* Here start "meaningful statements" *)
+
+
+(* 5 statements on inserting (helpers for mkGraph): update, insEdge, insEdges, insNode, insNodes *)
+Lemma _updateEntry_does_not_change_key_set : forall (node : Node) (f : NatSet.t * NatSet.t -> NatSet.t * NatSet.t) (ig : IG) (x : Node),
+  In x (IG_labNodes (_updateEntry node f ig)) <-> In x (IG_labNodes ig).
+Proof.
+  intros. unfold _updateEntry.
+  destruct (NatMap.find (elt:=NatSet.t * NatSet.t) node ig) eqn:isIn.
+  - rewrite _In_labNodes_is_InMap. rewrite _In_labNodes_is_InMap. rewrite WF.add_in_iff.
+    rewrite WF.in_find_iff. split.
+    + intros. destruct H.
+      -- rewrite <- H. rewrite isIn. unfold not. intros. discriminate H0.
+      -- assumption.
+    + intros. right. assumption.
+  - reflexivity.
+Qed.
+
+
+Lemma _insEdge_does_not_add_node : forall (edge : (Node * Node)) (ig : IG) (x : Node),
+  In x (IG_labNodes (_insEdge edge ig)) <-> In x (IG_labNodes ig).
+Proof.
+  intros. unfold _insEdge. destruct edge.
+  destruct (NatMap.mem (elt:=NatSet.t * NatSet.t) n ig && NatMap.mem (elt:=NatSet.t * NatSet.t) n0 ig) eqn:H0.
+  - rewrite _updateEntry_does_not_change_key_set.
+    rewrite _updateEntry_does_not_change_key_set.
+    reflexivity.
+  - reflexivity.
+Qed.
+
+
+Lemma _insEdges_does_not_add_nodes : forall (edges : list (Node * Node)) (ig : IG) (x : Node),
+  In x (IG_labNodes (_insEdges edges ig)) <-> In x (IG_labNodes ig).
+Proof.
+  intros. simpl. induction edges.
+  - simpl. reflexivity.
+  - simpl. rewrite _insEdge_does_not_add_node. rewrite IHedges. reflexivity.
+Qed. 
+
+
+Lemma _insNode_any_ins_node : forall (node : Node) (ig : IG) (x : Node),
+  In x (IG_labNodes (_insNode node ig)) <-> In x (node :: IG_labNodes ig).
+Proof.
+  intros. simpl. unfold _insNode.
+  rewrite _In_labNodes_is_InMap. rewrite WF.add_in_iff.
+  rewrite _In_labNodes_is_InMap.
+  reflexivity.
+Qed.  
+
+
+Lemma _insNodes_any_ins_all_nodes : forall (nodes : list Node) (ig : IG) (x : Node),
+  In x (IG_labNodes (_insNodes nodes ig)) <-> In x (nodes ++ IG_labNodes ig).
+Proof.
+  intros. induction nodes.
+    - simpl. reflexivity.
+    - simpl. rewrite _insNode_any_ins_node. simpl. rewrite IHnodes. reflexivity.
+Qed.
+
+Lemma _insEdge_on_empty_is_empty : forall (edge : Node * Node),
+  _insEdge edge IG_empty = IG_empty.
+(* This proof is very similar to "insEdge_does_not_add_node", but using it here it is more complicated than just doing it again  *)
+Proof.
+  intros. unfold _insEdge. destruct edge.
+  destruct (NatMap.mem (elt:=NatSet.t * NatSet.t) n IG_empty && NatMap.mem (elt:=NatSet.t * NatSet.t) n0 IG_empty) eqn:cond.
+  - compute. reflexivity.
+  - reflexivity.
+Qed. 
+
+
+Lemma _insEdges_on_empty_is_empty : forall (edges : list (Node * Node)),
+  _insEdges edges IG_empty = IG_empty.
+(* This proof is very similar to "insEdges_does_not_add_nodes", but using it here it is more complicated than just doing it again  *)
+Proof.
+  intros. induction edges; simpl.
+  - reflexivity.
+  - rewrite IHedges. rewrite _insEdge_on_empty_is_empty. reflexivity.
+Qed.
+
+
+
+(* "big" statement: *)
+Theorem IG_mkGraph_any_ins_all_nodes : forall (nl : list Node) (el : list (Node * Node)) (x : Node),
+  In x (IG_labNodes (IG_mkGraph nl el)) <-> In x nl.
+Proof.
+  intros. unfold IG_mkGraph. rewrite _insEdges_does_not_add_nodes. rewrite _insNodes_any_ins_all_nodes.
+  rewrite app_nil_r. reflexivity.
+Qed.
+
+
+Theorem IG_empty_isEmpty : IG_isEmpty IG_empty = true.
+Proof.
+  compute. reflexivity.
+Qed.
+
+Theorem IG_labNodes_empty_nil : IG_labNodes IG_empty = [].
+Proof.
+  compute. reflexivity.
+Qed.
+
+
+Lemma _not_NatMap_Empty_is_empty_false : forall (A : Type) (m : NatMap.t A), not (NatMap.Empty m) <-> NatMap.is_empty m = false.
+Proof.
+  intros. unfold not. rewrite WF.is_empty_iff. destruct (NatMap.is_empty (elt:=A) m) eqn:cond.
+  - firstorder. congruence.
+  - firstorder. congruence.
+Qed.
+
+(* Think about enforcing non-emptiness of the list with (x::xs) *)
+Theorem  IG_non_empty_isEmpty_false : forall (nodes : list Node) (edges : list (Node * Node)),
+  length nodes <> 0 <-> IG_isEmpty ((IG_mkGraph nodes edges)) = false.
+Proof.
+  intros. unfold IG_isEmpty. rewrite <- _not_NatMap_Empty_is_empty_false. unfold not.
+  destruct nodes; simpl; unfold IG_mkGraph.
+  - firstorder.
+    apply H.
+    apply WP.elements_Empty.
+
+    rewrite _insEdges_on_empty_is_empty. compute. reflexivity.
+  - firstorder.
+    + apply WP.elements_Empty in H0.
+      assert (HH : not (exists e, InA (fun x el : Node * (NatSet.t * NatSet.t) => x = el) (n, e) [])). {
+        unfold not. intros. destruct H1. inversion H1.
+      }
+      rewrite <- _In_conditions_same in HH.
+
+      unfold not in HH. apply HH.
+      
+      pose proof WF.elements_in_iff.
+      edestruct H1.
+      rewrite H0 in H2.
+      apply H2.
+      
+      apply _In_labNodes_is_InMap.
+      apply IG_mkGraph_any_ins_all_nodes. simpl. left. reflexivity.
+    + congruence.
+Qed.
+
+
+
+Theorem IG_matsh_empty_is_nothing : forall (node : Node), IG_match node IG_empty = (None, IG_empty).
 Proof.
   intros. compute. reflexivity.
 Qed.
 
-Theorem spec2 : forall (A B : Type) (nl : list (LNode A)) (el : list (LEdge B)), labNodes (mkGraph nl el) = nl.
+
+Theorem IG_spec4 : forall (node : Node) (nodes : list Node) (edges : list (Node * Node)), 
+  In node nodes -> exists froms tos, IG_match node (IG_mkGraph nodes edges) =
+  (Some (froms, tos), IG_mkGraph (filter (fun n => negb (node =? n)) nodes) (filter (fun '(from, to) => negb ((from =? node) || (to =? node))) edges)).
+(* This is not even a complete specification and it looks like a hard one to prove... *)
 Proof.
-  intros. compute.
+  intros.
+  
 Admitted.
 
-Theorem spec3 : forall (A B : Type) (n : node), matsh n (@empty A B) = (None, empty).
+
+Theorem IG_spec5 : forall (node : Node) (nodes : list Node) (edges : list (Node * Node)), 
+  not (In node nodes) -> IG_match node (IG_mkGraph nodes edges) = (None, IG_mkGraph nodes edges).
 Proof.
-  intros. compute.
 Admitted.
 
-Theorem spec4 : forall (A B : Type) (n : LNode A) (nl : list (LNode A)) (el : list (LEdge B)), 
-  In n nl -> exists map1 map2, matsh (fst n) (mkGraph nl el) =
-  (Some ((map1), snd n, (map2)), mkGraph (filter (fun '(idx, lab) => negb (fst n =? idx)) nl) (filter (fun '(to, from, lab) => negb ((to =? fst n) || (from =? fst n))) el)).
-(* This is not even a complete specification and it looks like a nightmare to prove... *)
-Admitted.
 
-Theorem spec5 : forall (A B : Type) (n : LNode A) (nl : list (LNode A)) (el : list (LEdge B)), 
-  not (In n nl) -> matsh (fst n) (mkGraph nl el) = (None, mkGraph nl el).
-Admitted.
+
 
 
 
@@ -128,3 +316,31 @@ Definition _valid_cond {A B : Type} (IG_data : NatMap.t (Context' A B)) : Prop :
 
 Definition IG_data_unsafe (A B : Type) : Type :=
   NatMap.t (Context' A B).
+
+
+
+(* Advanced theory *)
+
+  gmap f . gmap f 0 = gmap (f . f 0 )
+grev . grev = id
+
+We can prove gmap fusion by induction on the graph structure. For g = Empty we
+have by definition gmap f (gmap f 0 Empty) = gmap f Empty = Empty = gmap (f . f 0 )
+Empty. Otherwise, with g = c & g 0 we conclude by induction:
+gmap f (gmap f 0 g) = gmap f (gmap f 0 (c & g 0 ))
+= gmap f (f 0 c & (gmap f 0 g 0 ))
+= f (f 0 c) & gmap f (gmap f 0 g 0 )
+= (f . f 0 ) c & gmap (f . f 0 ) g 0
+= gmap (f . f 0 ) (c & g 0 )
+= gmap (f . f 0 ) g
+
+
+swap . swap = id
+gmap id = id
+
+
+
+grev . grev = gmap swap . gmap swap
+= gmap (swap . swap)
+= gmap id
+= id *)
